Spliting a module in two modules.

core/Semantics.v
@@ -42,9 +42,7 @@ Definition instantiateOnPattern (tr: Transformation) (sm : SourceModel) (sp: lis
 
 
 
-(** * Trace **)
-
-(** ** Building traces *)
+(** * Building traces *)
 
 Definition traceElementOnPattern (o: OutputPatternUnit) (sm: SourceModel) (sp: list SourceElementType) (iter: nat)
   : option TraceLink :=
@@ -70,37 +68,6 @@ Definition trace (tr: Transformation) (sm : SourceModel) : list TraceLink :=
   flat_map (traceOnPattern tr sm) (allTuples tr sm).  
 
 
-(** ** User read access in traces ([resolve]) *)
-
-Definition resolveIter (tls: list TraceLink) (sm: SourceModel) (name: string)
-            (sp: list SourceElementType)
-            (iter : nat) : option TargetElementType :=
-  option_map TraceLink.target (find (source_compare (sp,iter,name)) tls) .
-
-Definition resolve (tr: list TraceLink) (sm: SourceModel) (name: string)
-  (sp: list SourceElementType) : option TargetElementType :=
-  resolveIter tr sm name sp 0.
-
-
-Definition resolveAllIter (tr: list TraceLink) (sm: SourceModel) (name: string)
-  (sps: list(list SourceElementType)) (iter: nat)
-  : option (list TargetElementType) :=
-  Some (flat_map (fun l:(list SourceElementType) => optionToList (resolveIter tr sm name l iter)) sps).
-
-Definition resolveAll (tr: list TraceLink) (sm: SourceModel) (name: string)
-  (sps: list(list SourceElementType)) : option (list TargetElementType) :=
-  resolveAllIter tr sm name sps 0.
-
-Definition maybeResolve (tr: list TraceLink) (sm: SourceModel) (name: string)
-  (sp: option (list SourceElementType)) : option TargetElementType :=
-  sp' <- sp ;
-  resolve tr sm name sp' .
-
-
-Definition maybeResolveAll (tr: list TraceLink) (sm: SourceModel) (name: string)
-  (sp: option (list (list SourceElementType))) : option (list TargetElementType) :=
-  sp' <- sp ; 
-  resolveAll tr sm name sp'.
 
 
 (** * Apply link part of the r.h.s of rules (with traces) **)
@@ -139,29 +106,7 @@ End Semantics.
 (** * Some tactics *)
 
 (* tactics need to be outside the section to be visible *)
-Ltac inv_maybeResolve H := 
-  OptionUtils.monadInvN maybeResolve H.
 
-Ltac inv_maybeResolveAll H := 
-  OptionUtils.monadInvN maybeResolveAll H.
-
-
-Ltac inv_resolve H :=
-  match type of H with
-  | resolve _ _ _ _ = Some _ =>
-      unfold resolve in H ; 
-      OptionUtils.monadInvN resolveIter H
-  end.
-
-Ltac progress_maybeResolve H :=
-  match type of H with 
-    maybeResolve _ _ _ _ = Some _ =>
-      inv_maybeResolve H ;
-      inv_resolve H ; 
-      apply List.find_some in H ; 
-      let N := fresh H in
-      destruct H as (H & N)
-end.
 
 Ltac exploit_in_allTuples H :=
   match type of H with 
