core/Certification.v
@@ -10,6 +10,7 @@ Require Import core.Model.
 Require Import core.Engine.
 Require Import core.Syntax.
 Require Import core.Semantics.
+Require Import core.Resolve.
 Require Import core.Metamodel.
 Require Import core.TransformationConfiguration.
 Require Import core.SyntaxCertification.
