core/Resolve.v
@@ -1,0 +1,74 @@
+Require Import Semantics.
+
+Import String List Utils.
+Import core.TraceLink core.TransformationConfiguration.
+
+
+(** ** User read access in traces ([resolve]) *)
+
+Section Resolve.
+
+Context {tc: TransformationConfiguration}.
+
+Definition resolveIter (tls: list TraceLink) (sm: SourceModel) (name: string)
+            (sp: list SourceElementType)
+            (iter : nat) : option TargetElementType :=
+  option_map TraceLink.target (find (source_compare (sp,iter,name)) tls) .
+
+Definition resolve (tr: list TraceLink) (sm: SourceModel) (name: string)
+  (sp: list SourceElementType) : option TargetElementType :=
+  resolveIter tr sm name sp 0.
+
+
+Definition resolveAllIter (tr: list TraceLink) (sm: SourceModel) (name: string)
+  (sps: list(list SourceElementType)) (iter: nat)
+  : option (list TargetElementType) :=
+  Some (flat_map (fun l:(list SourceElementType) => optionToList (resolveIter tr sm name l iter)) sps).
+
+Definition resolveAll (tr: list TraceLink) (sm: SourceModel) (name: string)
+  (sps: list(list SourceElementType)) : option (list TargetElementType) :=
+  resolveAllIter tr sm name sps 0.
+
+Definition maybeResolve (tr: list TraceLink) (sm: SourceModel) (name: string)
+  (sp: option (list SourceElementType)) : option TargetElementType :=
+  sp' <- sp ;
+  resolve tr sm name sp' .
+
+
+Definition maybeResolveAll (tr: list TraceLink) (sm: SourceModel) (name: string)
+  (sp: option (list (list SourceElementType))) : option (list TargetElementType) :=
+  sp' <- sp ; 
+  resolveAll tr sm name sp'.
+
+
+End Resolve.
+
+(** * Some tactics *)
+
+(* tactics need to be outside the section to be visible *)
+
+Ltac inv_maybeResolve H := 
+  OptionUtils.monadInvN maybeResolve H.
+
+Ltac inv_maybeResolveAll H := 
+  OptionUtils.monadInvN maybeResolveAll H.
+
+
+Ltac inv_resolve H :=
+  match type of H with
+  | resolve _ _ _ _ = Some _ =>
+      unfold resolve in H ; 
+      OptionUtils.monadInvN resolveIter H
+  end.
+
+
+Ltac progress_maybeResolve H :=
+  match type of H with 
+    maybeResolve _ _ _ _ = Some _ =>
+      inv_maybeResolve H ;
+      inv_resolve H ; 
+      apply List.find_some in H ; 
+      let N := fresh H in
+      destruct H as (H & N)
+end.
+
